@prefix : <http://www.semanticweb.org/mehul/ontologies/2024/10/untitled-ontology-25/> .
@prefix owl: <http://www.w3.org/2002/07/owl#> .
@prefix rdf: <http://www.w3.org/1999/02/22-rdf-syntax-ns#> .
@prefix xml: <http://www.w3.org/XML/1998/namespace> .
@prefix xsd: <http://www.w3.org/2001/XMLSchema#> .
@prefix rdfs: <http://www.w3.org/2000/01/rdf-schema#> .
@base <http://www.semanticweb.org/mehul/ontologies/2024/10/untitled-ontology-25/> .

<https://www.dei.unipd.it/lodb/Cricketontology> rdf:type owl:Ontology ;
                                                 owl:imports <http://www.w3.org/2004/02/skos/core> ;
                                                 rdfs:comment """This is the Cricket Ontology created by group LODB.
We have taken the Women's T20 Cricket data from cricsheet to model the ontology."""@en ;
                                                 rdfs:label "Cricket Ontology by LODB"@en .

#################################################################
#    Object Properties
#################################################################

###  http://www.semanticweb.org/mehul/ontologies/2024/10/untitled-ontology-25/belongsToTeam
:belongsToTeam rdf:type owl:ObjectProperty ;
               owl:inverseOf :hasPlayer ;
               rdf:type owl:FunctionalProperty ;
               rdfs:domain :Player ;
               rdfs:range :Team ;
               rdfs:comment "It represents an object property that links player with the team."@en ;
               rdfs:label "belongsToTeam"@en .


###  http://www.semanticweb.org/mehul/ontologies/2024/10/untitled-ontology-25/hasBattingTeam
:hasBattingTeam rdf:type owl:ObjectProperty ,
                         owl:FunctionalProperty ,
                         owl:InverseFunctionalProperty ;
                rdfs:domain :Innings ;
                rdfs:range :Team ;
                rdfs:comment "Its an object property for innings. It represents that it has a batting team."@en ;
                rdfs:label "hasBattingTeam"@en .


###  http://www.semanticweb.org/mehul/ontologies/2024/10/untitled-ontology-25/hasDelivery
:hasDelivery rdf:type owl:ObjectProperty ,
                      owl:FunctionalProperty ;
             rdfs:domain :Innings ;
             rdfs:range :Delivery ;
             rdfs:comment "It represents balls played within the innings. Our data contains ball by ball data as delivery."@en ;
             rdfs:label "hasDelivery"@en .


###  http://www.semanticweb.org/mehul/ontologies/2024/10/untitled-ontology-25/hasFirstInning
:hasFirstInning rdf:type owl:ObjectProperty ;
                owl:inverseOf :isFirstInningOfMatch ;
                rdfs:domain :Match ;
                rdfs:range :Inning1 ;
                rdfs:comment "It links first innings with the match. Each match has two innings."@en ;
                rdfs:label "hasFirstInning"@en .


###  http://www.semanticweb.org/mehul/ontologies/2024/10/untitled-ontology-25/hasOutcome
:hasOutcome rdf:type owl:ObjectProperty ,
                     owl:FunctionalProperty ;
            rdfs:domain :Match ;
            rdfs:range :Outcome ;
            rdfs:comment "Its a Property that links a Match class with the  Outcome class."@en ;
            rdfs:label "hasOutcome"@en .


###  http://www.semanticweb.org/mehul/ontologies/2024/10/untitled-ontology-25/hasOutcomeToss
:hasOutcomeToss rdf:type owl:ObjectProperty ,
                         owl:FunctionalProperty ;
                rdfs:domain :Match ;
                rdfs:range :Toss ;
                rdfs:label "It represnts a property that links match with toss outcome."@en ,
                           "hasOutcomeToss"@en .


###  http://www.semanticweb.org/mehul/ontologies/2024/10/untitled-ontology-25/hasPlayer
:hasPlayer rdf:type owl:ObjectProperty ;
           rdfs:domain :Team ;
           rdfs:range :Player ;
           rdfs:comment "It represents the property that links team with the player. It is inverse of another property belongToTeam which shows relation of player with team."@en ;
           rdfs:label "hasPlayer"@en .


###  http://www.semanticweb.org/mehul/ontologies/2024/10/untitled-ontology-25/hasSecondInning
:hasSecondInning rdf:type owl:ObjectProperty ;
                 owl:inverseOf :isSecondInningOfMatch ;
                 rdfs:domain :Match ;
                 rdfs:range :Inning2 ;
                 rdfs:comment "It links Innings2 class with of  the match class. Every match has two innings"@en ;
                 rdfs:label "hasSecondInnings"@en .


###  http://www.semanticweb.org/mehul/ontologies/2024/10/untitled-ontology-25/hasWinner
:hasWinner rdf:type owl:ObjectProperty ,
                    owl:FunctionalProperty ;
           rdfs:domain :Toss ;
           rdfs:range :Team ;
           rdfs:comment "Its links toss decision with the team. Data contains toss winner teams for every innings."@en ;
           rdfs:label "hasWinner"@en .


###  http://www.semanticweb.org/mehul/ontologies/2024/10/untitled-ontology-25/isFirstInningOfMatch
:isFirstInningOfMatch rdf:type owl:ObjectProperty ;
                      rdfs:domain :Inning1 ;
                      rdfs:range :Match ;
                      rdfs:comment "Its a property of first innings which represents that it belongs to a match."@en ;
                      rdfs:label "isFirstInningsOfMatch"@en .


###  http://www.semanticweb.org/mehul/ontologies/2024/10/untitled-ontology-25/isOfficiatedBy
:isOfficiatedBy rdf:type owl:ObjectProperty ;
                owl:inverseOf :officiatedInMatch ;
                rdfs:domain :Match ;
                rdfs:range :Umpire ;
                rdfs:comment "It links match with the umpire. It has inverse property officiatedInMatch, that links umpire with match."@en ;
                rdfs:label "isOfficiatedBy"@en .


###  http://www.semanticweb.org/mehul/ontologies/2024/10/untitled-ontology-25/isParticipatedBy
:isParticipatedBy rdf:type owl:ObjectProperty ;
                  rdfs:domain :Match ;
                  rdfs:range :Team ;
                  rdfs:comment "It links team with the match. it represents those teams that participate in the match."@en ;
                  rdfs:label "isParticipatedBy"@en .


###  http://www.semanticweb.org/mehul/ontologies/2024/10/untitled-ontology-25/isSecondInningOfMatch
:isSecondInningOfMatch rdf:type owl:ObjectProperty ;
                       rdfs:domain :Inning2 ;
                       rdfs:range :Match ;
                       rdfs:comment "Its a property of second innings which represents that it belongs to a match."@en ;
                       rdfs:label "isSecondInningsOfMatch"@en .


###  http://www.semanticweb.org/mehul/ontologies/2024/10/untitled-ontology-25/officiatedInMatch
:officiatedInMatch rdf:type owl:ObjectProperty ;
                   rdfs:domain :Umpire ;
                   rdfs:range :Match ;
                   rdfs:comment "it represents the property that links umpire with match. Its an inverse of is OfficiatedBy property that links match with umpire."@en ;
                   rdfs:label "officiatedInMatch"@en .


###  http://www.semanticweb.org/mehul/ontologies/2024/10/untitled-ontology-25/wonBy
:wonBy rdf:type owl:ObjectProperty ,
                owl:FunctionalProperty ;
       rdfs:domain :Win ;
       rdfs:range :Team ;
       rdfs:comment "Property that links a Win to the winning Team."@en ;
       rdfs:label "wonBy"@en .


#################################################################
#    Data properties
#################################################################

###  http://www.semanticweb.org/mehul/ontologies/2024/10/untitled-ontology-25/hasDates
:hasDates rdf:type owl:DatatypeProperty ;
          rdfs:domain :Match ;
          rdfs:range xsd:dateTime ;
          rdfs:comment "This property represents the date of the match. Every match had been played on certain date."@en ;
          rdfs:label "hasDates"@en .


###  http://www.semanticweb.org/mehul/ontologies/2024/10/untitled-ontology-25/hasDecision
:hasDecision rdf:type owl:DatatypeProperty ,
                      owl:FunctionalProperty ;
             rdfs:domain :Toss ;
             rdfs:range [ rdf:type rdfs:Datatype ;
                          owl:oneOf [ rdf:type rdf:List ;
                                      rdf:first "bat" ;
                                      rdf:rest [ rdf:type rdf:List ;
                                                 rdf:first "field" ;
                                                 rdf:rest rdf:nil
                                               ]
                                    ]
                        ] ;
             rdfs:comment "It represents a decison outcome of toss, the winner team either chooses to bat or field, so it has two values."@en ;
             rdfs:label "hasDecision"@en .


###  http://www.semanticweb.org/mehul/ontologies/2024/10/untitled-ontology-25/hasManofMatch
:hasManofMatch rdf:type owl:DatatypeProperty ,
                        owl:FunctionalProperty ;
               rdfs:domain :Match ;
               rdfs:range xsd:string ;
               rdfs:comment "This property represents player who got man of the match title. It will show the name of player (if any) got this title in a particular match."@en ;
               rdfs:label "hasManofMatch"@en .


###  http://www.semanticweb.org/mehul/ontologies/2024/10/untitled-ontology-25/hasTotalBalls
:hasTotalBalls rdf:type owl:DatatypeProperty ;
               rdfs:domain :Delivery ;
               rdfs:range [ rdf:type rdfs:Datatype ;
                            owl:onDatatype xsd:integer ;
                            owl:withRestrictions ( [ xsd:minInclusive 120
                                                   ]
                                                   [ xsd:maxInclusive 125
                                                   ]
                                                 )
                          ] ;
               rdfs:comment "This property represents the total number of balls played during a match. In a single T20 match total balls are 120. Considering 5 wide/no balls, its range has been set from 120 to 125 inclusive."@en ;
               rdfs:label "hasTotalBalls"@en .


###  http://www.semanticweb.org/mehul/ontologies/2024/10/untitled-ontology-25/hasVenue
:hasVenue rdf:type owl:DatatypeProperty ,
                   owl:FunctionalProperty ;
          rdfs:domain :Match ;
          rdfs:range xsd:string ;
          rdfs:comment "The property hasVenue represents the location where the match was played. Its a string and shows the names of cricket grounds."@en ;
          rdfs:label "hasVenue"@en .


###  http://www.semanticweb.org/mehul/ontologies/2024/10/untitled-ontology-25/runs
:runs rdf:type owl:DatatypeProperty ,
               owl:FunctionalProperty ;
      rdfs:domain :Win ;
      rdfs:range xsd:integer ;
      rdfs:comment "Number of runs by which a match has been won" ;
      rdfs:label "runs"@en .


###  http://www.semanticweb.org/mehul/ontologies/2024/10/untitled-ontology-25/wickets
:wickets rdf:type owl:DatatypeProperty ,
                  owl:FunctionalProperty ;
         rdfs:domain :Win ;
         rdfs:range xsd:integer ;
         rdfs:comment "Number of wickets by which a match has been won" ;
         rdfs:label "wickets"@en .


#################################################################
#    Classes
#################################################################

###  http://www.semanticweb.org/mehul/ontologies/2024/10/untitled-ontology-25/Delivery
:Delivery rdf:type owl:Class ;
          owl:equivalentClass [ rdf:type owl:Restriction ;
                                owl:onProperty :hasTotalBalls ;
                                owl:qualifiedCardinality "1"^^xsd:nonNegativeInteger ;
                                owl:onDataRange xsd:integer
                              ] ;
          rdfs:comment "This is the class that holds the total number of balls in each inning."@en ;
          rdfs:label "Delivery"@en .


###  http://www.semanticweb.org/mehul/ontologies/2024/10/untitled-ontology-25/Inning1
:Inning1 rdf:type owl:Class ;
         rdfs:subClassOf :Innings ,
                         [ rdf:type owl:Restriction ;
                           owl:onProperty :hasDelivery ;
                           owl:someValuesFrom :Delivery
                         ] ,
                         [ rdf:type owl:Restriction ;
                           owl:onProperty :hasBattingTeam ;
                           owl:qualifiedCardinality "1"^^xsd:nonNegativeInteger ;
                           owl:onClass :Team
                         ] ;
         owl:disjointWith :Inning2 ;
         rdfs:comment "This class represents first innings in a cricket match, which is a phase of play during which one team bats and other team bowls depending on the toss decision."@en ;
         rdfs:label "Innings1"@en .


###  http://www.semanticweb.org/mehul/ontologies/2024/10/untitled-ontology-25/Inning2
:Inning2 rdf:type owl:Class ;
         rdfs:subClassOf :Innings ,
                         [ rdf:type owl:Restriction ;
                           owl:onProperty :hasDelivery ;
                           owl:someValuesFrom :Delivery
                         ] ,
                         [ rdf:type owl:Restriction ;
                           owl:onProperty :hasBattingTeam ;
                           owl:qualifiedCardinality "1"^^xsd:nonNegativeInteger ;
                           owl:onClass :Team
                         ] ;
         rdfs:comment "This class represents second innings of the match, where the team batting second attempts to chase the target set by batting team first."@en ;
         rdfs:label "Innings2"@en .


###  http://www.semanticweb.org/mehul/ontologies/2024/10/untitled-ontology-25/Innings
:Innings rdf:type owl:Class .


###  http://www.semanticweb.org/mehul/ontologies/2024/10/untitled-ontology-25/Match
:Match rdf:type owl:Class ;
       rdfs:subClassOf [ rdf:type owl:Restriction ;
                         owl:onProperty :isOfficiatedBy ;
                         owl:allValuesFrom :Umpire
                       ] ,
                       [ rdf:type owl:Restriction ;
                         owl:onProperty :hasOutcome ;
                         owl:qualifiedCardinality "1"^^xsd:nonNegativeInteger ;
                         owl:onClass :Outcome
                       ] ,
                       [ rdf:type owl:Restriction ;
                         owl:onProperty :isOfficiatedBy ;
                         owl:qualifiedCardinality "2"^^xsd:nonNegativeInteger ;
                         owl:onClass :Umpire
                       ] ,
                       [ rdf:type owl:Restriction ;
                         owl:onProperty :isParticipatedBy ;
                         owl:qualifiedCardinality "2"^^xsd:nonNegativeInteger ;
                         owl:onClass :Team
                       ] ;
       owl:disjointWith :Outcome ,
                        :Win ;
       rdfs:comment "This is the class Match that holds all the details about a particular match."@en ;
       rdfs:label "Match"@en .


###  http://www.semanticweb.org/mehul/ontologies/2024/10/untitled-ontology-25/Outcome
:Outcome rdf:type owl:Class ;
         owl:disjointWith :Team ;
         rdfs:comment "This class represents the outcome of the matches" .


###  http://www.semanticweb.org/mehul/ontologies/2024/10/untitled-ontology-25/Person
:Person rdf:type owl:Class .


###  http://www.semanticweb.org/mehul/ontologies/2024/10/untitled-ontology-25/Player
:Player rdf:type owl:Class ;
        owl:equivalentClass [ rdf:type owl:Restriction ;
                              owl:onProperty :belongsToTeam ;
                              owl:qualifiedCardinality "1"^^xsd:nonNegativeInteger ;
                              owl:onClass :Team
                            ] ;
        rdfs:subClassOf :Person ;
        owl:disjointWith :Umpire ;
        rdfs:comment "This class represents all the players participating in the game" ;
        rdfs:label "Player" .


###  http://www.semanticweb.org/mehul/ontologies/2024/10/untitled-ontology-25/Team
:Team rdf:type owl:Class ;
      owl:equivalentClass [ rdf:type owl:Restriction ;
                            owl:onProperty :hasPlayer ;
                            owl:someValuesFrom :Player
                          ] ,
                          [ rdf:type owl:Restriction ;
                            owl:onProperty :hasPlayer ;
                            owl:qualifiedCardinality "11"^^xsd:nonNegativeInteger ;
                            owl:onClass :Player
                          ] ;
      owl:disjointWith :Win ;
      rdfs:comment "This is the class that represents the 2 teams participating in the Cricket match" ;
      rdfs:label "Team"@en .


###  http://www.semanticweb.org/mehul/ontologies/2024/10/untitled-ontology-25/Toss
:Toss rdf:type owl:Class ;
      owl:equivalentClass [ rdf:type owl:Restriction ;
                            owl:onProperty :hasWinner ;
                            owl:qualifiedCardinality "1"^^xsd:nonNegativeInteger ;
                            owl:onClass :Team
                          ] ,
                          [ rdf:type owl:Restriction ;
                            owl:onProperty :hasDecision ;
                            owl:cardinality "1"^^xsd:nonNegativeInteger
                          ] ;
      rdfs:comment """Toss identifies the team that has won in the toss and also what the winning team chooses to deliver. 
For example, for the match India vs Australia, India wins the toss, and chooses to Field. 
Toss holds - India, Field"""@en ;
      rdfs:label "Toss"@en .


###  http://www.semanticweb.org/mehul/ontologies/2024/10/untitled-ontology-25/Umpire
:Umpire rdf:type owl:Class ;
        owl:equivalentClass [ rdf:type owl:Restriction ;
                              owl:onProperty :officiatedInMatch ;
                              owl:someValuesFrom :Match
                            ] ;
        rdfs:subClassOf :Person ;
        rdfs:comment "This class represents all the umpires in the game" ;
        rdfs:label "Umpire"@en .


###  http://www.semanticweb.org/mehul/ontologies/2024/10/untitled-ontology-25/Win
:Win rdf:type owl:Class ;
     owl:equivalentClass [ rdf:type owl:Restriction ;
                           owl:onProperty :wonBy ;
                           owl:qualifiedCardinality "1"^^xsd:nonNegativeInteger ;
                           owl:onClass :Team
                         ] ;
     rdfs:subClassOf :Outcome ;
     owl:disjointWith <http://www.w3.org/2004/02/skos/core#Concept> ;
     rdfs:comment "This class describes the wins (if that's the outcome)" .


#################################################################
#    Individuals
#################################################################

###  http://www.semanticweb.org/mehul/ontologies/2024/10/untitled-ontology-25/Australia
:Australia rdf:type owl:NamedIndividual ,
                    :Team ;
           owl:differentFrom :England ,
                             :India .


###  http://www.semanticweb.org/mehul/ontologies/2024/10/untitled-ontology-25/BF_Bowden
:BF_Bowden rdf:type owl:NamedIndividual ,
                    :Umpire ;
           owl:differentFrom :Kim_Cotton .


###  http://www.semanticweb.org/mehul/ontologies/2024/10/untitled-ontology-25/B_Biza
:B_Biza rdf:type owl:NamedIndividual ,
                 :Player ;
        owl:differentFrom :K_Ndlovu ;
        :belongsToTeam :Zimbabwe .


###  http://www.semanticweb.org/mehul/ontologies/2024/10/untitled-ontology-25/B_Cooper
:B_Cooper rdf:type owl:NamedIndividual ,
                   :Player ;
          owl:differentFrom :SS_Connell ;
          :belongsToTeam :West_indies .


###  http://www.semanticweb.org/mehul/ontologies/2024/10/untitled-ontology-25/Charles_Kariuki
:Charles_Kariuki rdf:type owl:NamedIndividual ,
                          :Umpire ;
                 owl:differentFrom :D_Odhiambo ,
                                   :someumpire .


###  http://www.semanticweb.org/mehul/ontologies/2024/10/untitled-ontology-25/D_Odhiambo
:D_Odhiambo rdf:type owl:NamedIndividual ,
                     :Umpire ;
            owl:differentFrom :someumpire .


###  http://www.semanticweb.org/mehul/ontologies/2024/10/untitled-ontology-25/Del1_m1
:Del1_m1 rdf:type owl:NamedIndividual ,
                  :Delivery ;
         owl:differentFrom :Del2_m1 ;
         :hasTotalBalls 120 .


###  http://www.semanticweb.org/mehul/ontologies/2024/10/untitled-ontology-25/Del2_m1
:Del2_m1 rdf:type owl:NamedIndividual ,
                  :Delivery ;
         :hasTotalBalls 122 .


###  http://www.semanticweb.org/mehul/ontologies/2024/10/untitled-ontology-25/England
:England rdf:type owl:NamedIndividual ,
                  :Team ;
         owl:differentFrom :India .


###  http://www.semanticweb.org/mehul/ontologies/2024/10/untitled-ontology-25/India
:India rdf:type owl:NamedIndividual ,
                :Team ;
       owl:differentFrom :Namibia ,
                         :Zimbabwe .


###  http://www.semanticweb.org/mehul/ontologies/2024/10/untitled-ontology-25/Inn1_m1
:Inn1_m1 rdf:type owl:NamedIndividual ,
                  :Inning1 ;
         owl:differentFrom :Inn2_m1 ;
         :hasBattingTeam :Namibia ;
         :hasDelivery :Del1_m1 .


###  http://www.semanticweb.org/mehul/ontologies/2024/10/untitled-ontology-25/Inn1_m3
:Inn1_m3 rdf:type owl:NamedIndividual ,
                  :Inning1 ;
         :hasBattingTeam :New_Zealand ;
         :isFirstInningOfMatch :Match3 ;
         :hasTotalBalls 122 .


###  http://www.semanticweb.org/mehul/ontologies/2024/10/untitled-ontology-25/Inn2_m1
:Inn2_m1 rdf:type owl:NamedIndividual ,
                  :Inning2 ;
         :hasBattingTeam :Zimbabwe ;
         :hasDelivery :Del2_m1 ;
         rdfs:comment "Inning2 for Match1" .


###  http://www.semanticweb.org/mehul/ontologies/2024/10/untitled-ontology-25/Inn2_m3
:Inn2_m3 rdf:type owl:NamedIndividual ,
                  :Inning2 ;
         :hasBattingTeam :West_indies ;
         :isSecondInningOfMatch :Match3 ;
         :hasTotalBalls 124 .


###  http://www.semanticweb.org/mehul/ontologies/2024/10/untitled-ontology-25/Jonathan
:Jonathan rdf:type owl:NamedIndividual ,
                   :Player ;
          :belongsToTeam :Australia .


###  http://www.semanticweb.org/mehul/ontologies/2024/10/untitled-ontology-25/K_Ndlovu
:K_Ndlovu rdf:type owl:NamedIndividual ,
                   :Player ;
          :belongsToTeam :Zimbabwe .


###  http://www.semanticweb.org/mehul/ontologies/2024/10/untitled-ontology-25/Kim_Cotton
:Kim_Cotton rdf:type owl:NamedIndividual ,
                     :Umpire .


###  http://www.semanticweb.org/mehul/ontologies/2024/10/untitled-ontology-25/ML_Green
:ML_Green rdf:type owl:NamedIndividual ,
                   :Player ;
          owl:differentFrom :NC_Dodd ;
          :belongsToTeam :New_Zealand .


###  http://www.semanticweb.org/mehul/ontologies/2024/10/untitled-ontology-25/M_Short
:M_Short rdf:type owl:NamedIndividual ,
                  :Umpire ;
         owl:differentFrom :S_Loftie_Eaton ,
                           :someumpire .


###  http://www.semanticweb.org/mehul/ontologies/2024/10/untitled-ontology-25/Match1
:Match1 rdf:type owl:NamedIndividual ,
                 :Match ;
        owl:differentFrom :Match2 ,
                          :Match3 ;
        :hasOutcomeToss :Toss1 ;
        :isOfficiatedBy :D_Odhiambo ,
                        :M_Short ;
        :isParticipatedBy :Australia ,
                          :India ;
        :hasManofMatch "" ;
        :hasVenue "Venice" .


###  http://www.semanticweb.org/mehul/ontologies/2024/10/untitled-ontology-25/Match2
:Match2 rdf:type owl:NamedIndividual ,
                 :Match ;
        owl:differentFrom :Match3 ;
        :hasOutcomeToss :Toss2 ;
        :isOfficiatedBy :M_Short ,
                        :S_Loftie_Eaton ;
        :isParticipatedBy :Namibia ,
                          :Zimbabwe ;
        :hasManofMatch "" ;
        :hasVenue "Wanderers Cricket Ground, Windhoek" .


###  http://www.semanticweb.org/mehul/ontologies/2024/10/untitled-ontology-25/Match3
:Match3 rdf:type owl:NamedIndividual ,
                 :Match ;
        :hasOutcomeToss :Toss3 ;
        :isOfficiatedBy :BF_Bowden ,
                        :Kim_Cotton ;
        :isParticipatedBy :New_Zealand ,
                          :West_indies ;
        :hasManofMatch "HK Matthews" ;
        :hasVenue "Pukekura Park, New Zealand" .


###  http://www.semanticweb.org/mehul/ontologies/2024/10/untitled-ontology-25/NC_Dodd
:NC_Dodd rdf:type owl:NamedIndividual ,
                  :Player ;
         :belongsToTeam :New_Zealand .


###  http://www.semanticweb.org/mehul/ontologies/2024/10/untitled-ontology-25/Namibia
:Namibia rdf:type owl:NamedIndividual ,
                  :Team ;
         owl:differentFrom :Zimbabwe .


###  http://www.semanticweb.org/mehul/ontologies/2024/10/untitled-ontology-25/New_Zealand
:New_Zealand rdf:type owl:NamedIndividual ,
                      :Team ;
             owl:differentFrom :West_indies .


###  http://www.semanticweb.org/mehul/ontologies/2024/10/untitled-ontology-25/NoResult
:NoResult rdf:type owl:NamedIndividual ,
                   :Outcome ,
                   <http://www.w3.org/2004/02/skos/core#Concept> ;
          owl:differentFrom :Tie ;
          rdfs:comment "This a skos:Concept representing a no result as outcome of the match" .


###  http://www.semanticweb.org/mehul/ontologies/2024/10/untitled-ontology-25/SA_Wittman
:SA_Wittman rdf:type owl:NamedIndividual ;
            owl:differentFrom :Yasmeen_Khan ;
            :belongsToTeam :Namibia .


###  http://www.semanticweb.org/mehul/ontologies/2024/10/untitled-ontology-25/SS_Connell
:SS_Connell rdf:type owl:NamedIndividual ,
                     :Player ;
            :belongsToTeam :West_indies .


###  http://www.semanticweb.org/mehul/ontologies/2024/10/untitled-ontology-25/S_Loftie_Eaton
:S_Loftie_Eaton rdf:type owl:NamedIndividual ,
                         :Umpire ;
                owl:differentFrom :someumpire .


###  http://www.semanticweb.org/mehul/ontologies/2024/10/untitled-ontology-25/Tie
:Tie rdf:type owl:NamedIndividual ,
              :Outcome ,
              <http://www.w3.org/2004/02/skos/core#Concept> ;
     rdfs:comment "This a skos:Concept representing a tie as outcome of the match" .


###  http://www.semanticweb.org/mehul/ontologies/2024/10/untitled-ontology-25/Toss1
:Toss1 rdf:type owl:NamedIndividual ,
                :Toss ;
       owl:differentFrom :Toss2 ,
                         :Toss3 ;
       :hasWinner :India ;
       :hasDecision "bat" .


###  http://www.semanticweb.org/mehul/ontologies/2024/10/untitled-ontology-25/Toss2
:Toss2 rdf:type owl:NamedIndividual ,
                :Toss ;
       owl:differentFrom :Toss3 ;
       :hasWinner :Namibia ;
       :hasDecision "field" .


###  http://www.semanticweb.org/mehul/ontologies/2024/10/untitled-ontology-25/Toss3
:Toss3 rdf:type owl:NamedIndividual ,
                :Toss ;
       :hasWinner :West_indies ;
       :hasDecision "field" .


###  http://www.semanticweb.org/mehul/ontologies/2024/10/untitled-ontology-25/West_indies
:West_indies rdf:type owl:NamedIndividual .


###  http://www.semanticweb.org/mehul/ontologies/2024/10/untitled-ontology-25/Yasmeen_Khan
:Yasmeen_Khan rdf:type owl:NamedIndividual ,
                       :Player ;
              :belongsToTeam :Namibia .


###  http://www.semanticweb.org/mehul/ontologies/2024/10/untitled-ontology-25/Zimbabwe
:Zimbabwe rdf:type owl:NamedIndividual ,
                   :Team .


###  http://www.semanticweb.org/mehul/ontologies/2024/10/untitled-ontology-25/someumpire
:someumpire rdf:type owl:NamedIndividual ,
                     :Umpire .


###  Generated by the OWL API (version 4.5.29.2024-05-13T12:11:03Z) https://github.com/owlcs/owlapi
